src/QueryStructure/Refinements/Bags/BagsProperties.v
@@ -1,72 +1,64 @@
 Require Import BagsInterface AdditionalLemmas.
 Require Import AdditionalMorphisms.
 
-Lemma binsert_enumerate_weak {TContainer TItem TSearchTerm} {bag: Bag TContainer TItem TSearchTerm}:
-  forall item inserted container,
-    List.In item (benumerate (binsert container inserted)) <->
-    List.In item (benumerate container) \/ item = inserted.
-Proof.
-  intros.
-  rewrite <- refold_in.
-  apply in_permutation_morphism; eauto using binsert_enumerate. 
-Qed.
+Section BagsProperties.
 
-Lemma benumerate_empty_eq_nil {TContainer TItem TSearchTerm} (bag: Bag TContainer TItem TSearchTerm):
-  (benumerate bempty) = nil. 
-Proof.
-  pose proof (benumerate_empty) as not_in;
-  unfold BagEnumerateEmpty in not_in.
-  destruct (benumerate bempty) as [ | item ? ]; 
-    simpl in *;
-    [ | exfalso; apply (not_in item) ];
-    eauto.
-Qed.
+  Context {TContainer   : Type}
+          {TItem        : Type}
+          {TSearchTerm  : Type}
+          {TUpdateTerm  : Type}
+          {bag          : Bag TContainer TItem TSearchTerm TUpdateTerm}.
 
-Lemma binsert_enumerate_length :
-  forall {TItem TContainer TSearchTerm} {bag_proof: Bag TContainer TItem TSearchTerm},
-  forall (bag: TContainer) (item: TItem),
-    List.length (benumerate (binsert bag item)) = S (List.length (benumerate bag)).
-Proof.      
-  intros; rewrite binsert_enumerate; simpl; trivial.
-Qed.
+  Lemma binsert_enumerate_weak
+  : forall item inserted container,
+      List.In item (benumerate (binsert container inserted)) <->
+      List.In item (benumerate container) \/ item = inserted.
+  Proof.
+    intros.
+    rewrite <- refold_in.
+    apply in_permutation_morphism; eauto using binsert_enumerate.
+  Qed.
 
-Definition HasDecidableEquality (T: Type) :=
-  forall (x y: T), {x = y} + {x <> y}.
+  Lemma benumerate_empty_eq_nil
+  : benumerate bempty = nil.
+  Proof.
+    pose proof (benumerate_empty) as not_in;
+    unfold BagEnumerateEmpty in not_in.
+    destruct (benumerate bempty) as [ | item ? ];
+      simpl in *;
+      [ | exfalso; apply (not_in item) ];
+      eauto.
+  Qed.
 
-Definition _BagInsertCount
-           {TContainer TItem}
-           (benumerate : TContainer -> list TItem)
-           (binsert    : TContainer -> TItem -> TContainer)
-           (bcount     : HasDecidableEquality TItem -> TContainer -> TItem -> nat) :=
-  forall (beq : HasDecidableEquality TItem),
-  forall item inserted container,
-    bcount beq (binsert container inserted) item =
-    bcount beq container item + if beq item inserted then 1 else 0.
+  Lemma binsert_enumerate_length
+  : forall (bag: TContainer) (item: TItem),
+      List.length (benumerate (binsert bag item)) = S (List.length (benumerate bag)).
+  Proof.
+    intros; rewrite binsert_enumerate; simpl; trivial.
+  Qed.
 
-Definition _BagCountEmpty
-           {TContainer TItem: Type}
-           (benumerate : TContainer -> list TItem)
-           (bempty     : TContainer)
-           (bcount     : HasDecidableEquality TItem -> TContainer -> TItem -> nat) :=
-  forall (beq : HasDecidableEquality TItem),
-  forall item, bcount beq bempty item = 0. 
+  Definition _bcount container item :=
+    List.length (List.filter (fun x => if bfind_matcher item x then true else false) (benumerate container)).
 
-Definition _bcount {TContainer TItem TSearchTerm} (bag: Bag TContainer TItem TSearchTerm) 
-           (dec: HasDecidableEquality TItem) container item :=
-  List.length (List.filter (fun x => if dec item x then true else false) (benumerate container)). 
+  Definition _BagInsertCount :=
+    forall (search_term : TSearchTerm) (item : TItem) (container : TContainer),
+      _bcount (binsert container item) search_term =
+      _bcount container search_term + if bfind_matcher search_term item then 1 else 0.
 
-Lemma _bcount_empty {TContainer TItem TSearchTerm} :
-  forall (bag: Bag TContainer TItem TSearchTerm),
-    @_BagCountEmpty TContainer TItem benumerate bempty (_bcount bag).
-Proof.
-  unfold _BagCountEmpty, _bcount; intros;
-  rewrite benumerate_empty_eq_nil; simpl; trivial.
-Qed.
+  Definition _BagCountEmpty :=
+    forall item, _bcount bempty item = 0.
 
-Lemma _binsert_count {TContainer TItem TSearchTerm} :
-  forall (bag: Bag TContainer TItem TSearchTerm),
-    @_BagInsertCount TContainer TItem benumerate binsert (_bcount bag).
-Proof.
-  unfold _BagInsertCount, _bcount; intros;
-  rewrite binsert_enumerate; simpl; destruct (beq item inserted); simpl; omega.
-Qed.
+  Lemma _bcount_empty :
+      _BagCountEmpty.
+  Proof.
+    unfold _BagCountEmpty, _bcount; intros.
+    rewrite benumerate_empty_eq_nil; simpl; trivial.
+  Qed.
+
+  Lemma _binsert_count : _BagInsertCount.
+  Proof.
+    unfold _BagInsertCount, _bcount; intros;
+    rewrite binsert_enumerate; simpl; destruct (bfind_matcher search_term item); simpl; omega.
+  Qed.
+
+End BagsProperties.
