src/QueryStructure/Refinements/Bags/CountingListBags.v
@@ -3,266 +3,265 @@ Unset Implicit Arguments.
 
 Open Scope list.
 
-Record CountingList {A} :=
-  {
-    clength   : nat;
-    ccontents : list A;
-    cconsistent: List.length ccontents = clength
-  }.
+Section CountingListBags.
 
-Lemma empty_length {A} :
-  List.length (@nil A) = 0.
-Proof.
-  reflexivity.
-Qed.
+  Context {TItem : Type}.
 
-Definition CountingList_empty {TItem} : @CountingList TItem :=
-  {|
-    clength := 0;
-    ccontents := @nil TItem;
-    cconsistent := empty_length
-  |}.
+  Record CountingList :=
+    {
+      clength   : nat;
+      ccontents : list TItem;
+      cconsistent: List.length ccontents = clength
+    }.
 
-Fixpoint MatchAgainstMany {TItem}
-         (search_terms : list (TItem -> bool)) (item: TItem) :=
-  match search_terms with
-    | nil                      => true
-    | cons is_match more_terms => andb (is_match item) (MatchAgainstMany more_terms item)
-  end.
+  Lemma empty_length :
+    List.length (@nil TItem) = 0.
+  Proof.
+    reflexivity.
+  Qed.
 
-Definition CountingListAsBag_bfind
-           {TItem: Type}
-           (container: @CountingList TItem) (search_terms: list (TItem -> bool)) :=
-  match search_terms with
-    | nil                      => ccontents container
-    | cons is_match more_terms => List.filter (MatchAgainstMany search_terms) (ccontents container)
-  end.
+  Definition CountingList_empty : CountingList :=
+    {|
+      clength := 0;
+      ccontents := @nil TItem;
+      cconsistent := empty_length
+    |}.
 
-Lemma CountingList_insert :
-  forall (TItem : Type) (container : @CountingList TItem) (item : TItem),
-    length (item :: ccontents container) = S (clength container).
-Proof.
-  intros; rewrite <- (cconsistent container); reflexivity.
-Qed.
+  Fixpoint MatchAgainstMany
+           (search_terms : list (TItem -> bool)) 
+           (item: TItem) :=
+    match search_terms with
+      | nil                      => true
+      | cons is_match more_terms => andb (is_match item) (MatchAgainstMany more_terms item)
+    end.
 
-Definition CountingListAsBag_binsert
-           {TItem: Type}
-           (container: @CountingList TItem)
-           (item: TItem) : @CountingList TItem :=
-  {| clength := S (clength container);
-     ccontents := cons item (ccontents container);
-     cconsistent := CountingList_insert TItem container item |}.
+  Definition CountingListAsBag_bfind
+             (container: CountingList) 
+             (search_terms: list (TItem -> bool)) :=
+    match search_terms with
+      | nil                      => ccontents container
+      | cons is_match more_terms => List.filter (MatchAgainstMany search_terms) (ccontents container)
+    end.
 
-Definition CountingListAsBag_bcount
-           {TItem: Type}
-           (container: @CountingList TItem) (search_terms: list (TItem -> bool)) :=
-  match search_terms with
-    | nil => clength container
-    | _   => List.fold_left (fun acc x => acc + if (MatchAgainstMany search_terms x) then 1 else 0)
-                            (ccontents container) 0
-  end.
+  Lemma CountingList_insert :
+    forall (container : CountingList) (item : TItem),
+      length (item :: ccontents container) = S (clength container).
+  Proof.
+    intros; rewrite <- (cconsistent container); reflexivity.
+  Qed.
 
-Fixpoint CountingListPartition
-         {TItem: Type}
-         (contents : list TItem)
-         (search_term : TItem -> bool)
-: prod (@CountingList TItem) (@CountingList TItem) :=
-  match contents with
-    | nil => (CountingList_empty, CountingList_empty)
-    | x :: tl => let (g,d) := CountingListPartition tl search_term in
-                 if search_term x then
-                   (CountingListAsBag_binsert g x, d)
-                 else
-                   (g, CountingListAsBag_binsert d x)
-  end.
+  Definition CountingListAsBag_binsert
+             (container: CountingList)
+             (item: TItem) : CountingList :=
+    {| clength := S (clength container);
+       ccontents := cons item (ccontents container);
+       cconsistent := CountingList_insert container item |}.
 
-Definition CountingListAsBag_bdelete
-           {TItem : Type}
-           (container : @CountingList TItem)
-           (search_terms : list (TItem -> bool)) :=
-  snd (CountingListPartition (ccontents container) (MatchAgainstMany search_terms)).
+  Definition CountingListAsBag_bcount
+             (container: CountingList) 
+             (search_terms: list (TItem -> bool)) :=
+    match search_terms with
+      | nil => clength container
+      | _   => List.fold_left (fun acc x => acc + if (MatchAgainstMany search_terms x) then 1 else 0)
+                              (ccontents container) 0
+    end.
 
-Lemma CountingListMap_consistent
-      {TItem: Type}
-      (container: @CountingList TItem)
-      (update_f : TItem -> TItem)
-: length (List.map update_f (ccontents container)) = clength container.
-Proof.
-  rewrite List.map_length; auto using cconsistent.
-Qed.
+  Fixpoint CountingListPartition
+           (contents : list TItem)
+           (search_term : TItem -> bool)
+  : prod CountingList CountingList :=
+    match contents with
+      | nil => (CountingList_empty, CountingList_empty)
+      | x :: tl => let (g,d) := CountingListPartition tl search_term in
+                   if search_term x then
+                     (CountingListAsBag_binsert g x, d)
+                   else
+                     (g, CountingListAsBag_binsert d x)
+    end.
 
-Definition CountingListMap
-         {TItem: Type}
-         (container: @CountingList TItem)
-         (update_f : TItem -> TItem)
-: @CountingList TItem :=
-  {| clength := clength container;
-     ccontents := List.map update_f (ccontents container);
-     cconsistent := CountingListMap_consistent container update_f|}.
+  Definition CountingListAsBag_bdelete
+             (container : CountingList)
+             (search_terms : list (TItem -> bool)) :=
+    let (d, r) := (CountingListPartition (ccontents container) (MatchAgainstMany search_terms))
+    in (ccontents d, r).
 
-Lemma CountingListAsBag_Partition_App
-      {TItem : Type}
-      (container : @CountingList TItem)
-      (search_term : TItem -> bool)
-: length
-    (let (g, d) :=
-         CountingListPartition (ccontents container) search_term in
-     ccontents d ++ ccontents g) =
-  let (g, d) :=
-      CountingListPartition (ccontents container) search_term in
-  (clength g) + (clength d).
-Proof.
-  destruct container as [n l length_l]; simpl;
-  destruct (CountingListPartition l search_term); simpl.
-  rewrite List.app_length; repeat rewrite cconsistent; auto with arith.
-Qed.
+  Lemma CountingListMap_consistent
+        (container: CountingList)
+        (update_f : TItem -> TItem)
+  : length (List.map update_f (ccontents container)) = clength container.
+  Proof.
+    rewrite List.map_length; auto using cconsistent.
+  Qed.
 
-Lemma CountingListAsBag_bupdate_Consistent
-      {TItem : Type}
-      (container : @CountingList TItem)
-      (search_term : TItem -> bool)
-      (update_f : TItem -> TItem)
-: length
-    (let (g, d) :=
-         CountingListPartition (ccontents container) search_term in
-     ccontents d ++ List.map update_f (ccontents g)) =
-  clength container.
-Proof.
-  destruct container as [n l length_l]; simpl; revert n length_l;
-  induction l; simpl; intros; auto.
-  destruct (CountingListPartition l search_term); simpl.
-  erewrite <- length_l, <- (IHl (length l)); auto.
-  destruct (search_term a); simpl;
-  rewrite List.app_length; simpl; rewrite List.map_length;
-  repeat rewrite cconsistent; auto.
-  rewrite List.app_length; simpl; rewrite List.map_length;
-  repeat rewrite cconsistent; auto.
-Qed.
+  Definition CountingListMap
+             (container: CountingList)
+             (update_f : TItem -> TItem)
+  : CountingList :=
+    {| clength := clength container;
+       ccontents := List.map update_f (ccontents container);
+       cconsistent := CountingListMap_consistent container update_f|}.
 
-Program Definition CountingListAsBag_bupdate
-           {TItem : Type}
-           (container : @CountingList TItem)
-           (search_terms : list (TItem -> bool))
-           (update_f : TItem -> TItem) :
-  @CountingList TItem :=
-  {| clength := clength container;
-     ccontents :=
-       let (g, d) := (CountingListPartition (ccontents container)
-                                            (MatchAgainstMany search_terms)) in
-       (ccontents d) ++ (List.map update_f (ccontents g));
-     cconsistent := CountingListAsBag_bupdate_Consistent
-                      container
-                      (MatchAgainstMany search_terms)
-                      update_f
-  |}.
+  Lemma CountingListAsBag_Partition_App
+        (container : CountingList)
+        (search_term : TItem -> bool)
+  : length
+      (let (g, d) :=
+           CountingListPartition (ccontents container) search_term in
+       ccontents d ++ ccontents g) =
+    let (g, d) :=
+        CountingListPartition (ccontents container) search_term in
+    (clength g) + (clength d).
+  Proof.
+    destruct container as [n l length_l]; simpl;
+    destruct (CountingListPartition l search_term); simpl.
+    rewrite List.app_length; repeat rewrite cconsistent; auto with arith.
+  Qed.
 
-Lemma CountingList_BagInsertEnumerate :
-  forall {TItem: Type},
-  BagInsertEnumerate ccontents (CountingListAsBag_binsert (TItem := TItem)).
-Proof.
-  firstorder.
-Qed.
+  Lemma CountingListAsBag_bupdate_Consistent
+        (container : CountingList)
+        (search_term : TItem -> bool)
+        (update_f : TItem -> TItem)
+  : length
+      (let (g, d) :=
+           CountingListPartition (ccontents container) search_term in
+       ccontents d ++ List.map update_f (ccontents g)) =
+    clength container.
+  Proof.
+    destruct container as [n l length_l]; simpl; revert n length_l;
+    induction l; simpl; intros; auto.
+    destruct (CountingListPartition l search_term); simpl.
+    erewrite <- length_l, <- (IHl (length l)); auto.
+    destruct (search_term a); simpl;
+    rewrite List.app_length; simpl; rewrite List.map_length;
+    repeat rewrite cconsistent; auto.
+    rewrite List.app_length; simpl; rewrite List.map_length;
+    repeat rewrite cconsistent; auto.
+  Qed.
 
-Lemma CountingList_BagEnumerateEmpty :
-  forall {TItem: Type},
-    BagEnumerateEmpty ccontents (@CountingList_empty TItem).
-Proof.
-  firstorder.
-Qed.
+  Program Definition CountingListAsBag_bupdate
+          (container : CountingList)
+          (search_terms : list (TItem -> bool))
+          (update_f : TItem -> TItem) :
+    CountingList :=
+    {| clength := clength container;
+       ccontents :=
+         let (g, d) := (CountingListPartition (ccontents container)
+                                              (MatchAgainstMany search_terms)) in
+         (ccontents d) ++ (List.map update_f (ccontents g));
+       cconsistent := CountingListAsBag_bupdate_Consistent
+                        container
+                        (MatchAgainstMany search_terms)
+                        update_f
+    |}.
 
-Lemma CountingList_BagFindStar :
-  forall {TItem: Type},
-    BagFindStar (CountingListAsBag_bfind) (@ccontents TItem) nil.
-Proof.
-  firstorder.
-Qed.
+  Lemma CountingList_BagInsertEnumerate :
+      BagInsertEnumerate ccontents CountingListAsBag_binsert.
+  Proof.
+    firstorder.
+  Qed.
 
-Require Import AdditionalLemmas.
+  Lemma CountingList_BagEnumerateEmpty :
+    BagEnumerateEmpty ccontents CountingList_empty.
+  Proof.
+    firstorder.
+  Qed.
 
-Lemma CountingList_BagFindCorrect :
-  forall {TItem: Type},
-         BagFindCorrect CountingListAsBag_bfind (@MatchAgainstMany TItem) (ccontents).
-Proof.
-  destruct search_term; simpl; [ rewrite filter_all_true | ]; reflexivity.
-Qed.
+  Lemma CountingList_BagFindStar :
+      BagFindStar CountingListAsBag_bfind ccontents nil.
+  Proof.
+    firstorder.
+  Qed.
 
-Require Import Omega.
-Lemma CountingList_BagCountCorrect_aux :
-  forall {TItem: Type},
-  forall (container: list TItem) (search_term: list (TItem -> bool)) default,
-    length (List.filter (MatchAgainstMany search_term) container) + default =
-    List.fold_left
-      (fun (acc : nat) (x : TItem) =>
-         acc + (if MatchAgainstMany search_term x then 1 else 0))
-      container default.
-Proof.
-  induction container; intros.
+  Require Import AdditionalLemmas.
 
-  + trivial.
-  + simpl; destruct (MatchAgainstMany search_term a);
-    simpl; rewrite <- IHcontainer; omega.
-Qed.
+  Lemma CountingList_BagFindCorrect :
+      BagFindCorrect CountingListAsBag_bfind MatchAgainstMany ccontents.
+  Proof.
+    destruct search_term; simpl; [ rewrite filter_all_true | ]; reflexivity.
+  Qed.
 
-Lemma CountingList_BagCountCorrect :
-  forall {TItem: Type},
-    BagCountCorrect (TItem := TItem) (CountingListAsBag_bcount) (CountingListAsBag_bfind).
-Proof.
-  unfold BagCountCorrect, CountingListAsBag_bcount, CountingListAsBag_bfind; intros;
-  pose proof (CountingList_BagCountCorrect_aux (ccontents container) search_term 0) as temp;
-  rewrite plus_0_r in temp; simpl in temp;
-  destruct search_term; simpl; [ apply cconsistent | apply temp ].
-Qed.
+  Require Import Omega.
+  Lemma CountingList_BagCountCorrect_aux :
+    forall (container: list TItem) (search_term: list (TItem -> bool)) default,
+      length (List.filter (MatchAgainstMany search_term) container) + default =
+      List.fold_left
+        (fun (acc : nat) (x : TItem) =>
+           acc + (if MatchAgainstMany search_term x then 1 else 0))
+        container default.
+  Proof.
+    induction container; intros.
 
-Lemma CountingList_BagDeleteCorrect :
-  forall {TItem: Type},
-    BagDeleteCorrect (TItem := TItem) CountingListAsBag_bfind MatchAgainstMany ccontents
-                     CountingListAsBag_bdelete.
-Proof.
-  unfold BagDeleteCorrect; destruct container as [n l length_l];
-  revert n length_l; induction l; simpl; intros.
-  constructor.
-  pose proof (IHl _ (refl_equal _) search_term).
-  unfold CountingListAsBag_bdelete in *; simpl in *.
-  destruct (MatchAgainstMany search_term a);
-  destruct (CountingListPartition l (MatchAgainstMany search_term));
-  destruct (List.partition (MatchAgainstMany search_term) l); simpl; auto.
-Qed.
+    + trivial.
+    + simpl; destruct (MatchAgainstMany search_term a);
+      simpl; rewrite <- IHcontainer; omega.
+  Qed.
 
-Lemma CountingList_BagUpdateCorrect :
-  forall {TItem: Type},
-    BagUpdateCorrect (TItem := TItem) CountingListAsBag_bfind MatchAgainstMany ccontents
-                     CountingListAsBag_bupdate.
-Proof.
-  unfold BagUpdateCorrect; destruct container as [n l length_l];
-  revert n length_l; induction l; simpl; intros.
-  constructor.
-  pose proof (IHl _ (refl_equal _) search_term f_update).
-  unfold CountingListAsBag_bdelete in *; simpl in *.
-  destruct (MatchAgainstMany search_term a);
-  destruct (CountingListPartition l (MatchAgainstMany search_term));
-  destruct (List.partition (MatchAgainstMany search_term) l); simpl in *; auto.
-  rewrite Permutation_app_comm; simpl.
-  apply Permutation_cons_app; rewrite Permutation_app_comm; auto.
-Qed.
+  Lemma CountingList_BagCountCorrect :
+      BagCountCorrect CountingListAsBag_bcount CountingListAsBag_bfind.
+  Proof.
+    unfold BagCountCorrect, CountingListAsBag_bcount, CountingListAsBag_bfind; intros;
+    pose proof (CountingList_BagCountCorrect_aux (ccontents container) search_term 0) as temp;
+    rewrite plus_0_r in temp; simpl in temp;
+    destruct search_term; simpl; [ apply cconsistent | apply temp ].
+  Qed.
 
-Instance CountingListAsBag {TItem: Type}
-: Bag (@CountingList TItem) TItem (list (TItem -> bool)) :=
-  {|
-    bempty := CountingList_empty;
-    bstar  := nil;
+  Lemma CountingList_BagDeleteCorrect :
+      BagDeleteCorrect CountingListAsBag_bfind MatchAgainstMany ccontents
+                       CountingListAsBag_bdelete.
+  Proof.
+    unfold BagDeleteCorrect; destruct container as [n l length_l];
+    revert n length_l; induction l; simpl; intros; split.
+    + constructor.
+    + constructor.
+    + destruct (IHl _ (refl_equal _) search_term).
+      unfold CountingListAsBag_bdelete in *; simpl in *.
+      destruct (MatchAgainstMany search_term a);
+        destruct (CountingListPartition l (MatchAgainstMany search_term));
+        destruct (List.partition (MatchAgainstMany search_term) l); simpl; auto.
+    +  destruct (IHl _ (refl_equal _) search_term).
+      unfold CountingListAsBag_bdelete in *; simpl in *.
+      destruct (MatchAgainstMany search_term a);
+        destruct (CountingListPartition l (MatchAgainstMany search_term));
+        destruct (List.partition (MatchAgainstMany search_term) l); simpl; auto.
+  Qed.
 
-    benumerate := ccontents;
-    bfind      := CountingListAsBag_bfind;
-    binsert    := CountingListAsBag_binsert;
-    bcount     := CountingListAsBag_bcount;
-    bdelete    := CountingListAsBag_bdelete;
-    bupdate    := CountingListAsBag_bupdate;
+  Lemma CountingList_BagUpdateCorrect :
+      BagUpdateCorrect CountingListAsBag_bfind MatchAgainstMany ccontents
+                       id CountingListAsBag_bupdate.
+  Proof.
+    unfold BagUpdateCorrect; destruct container as [n l length_l];
+    revert n length_l; induction l; simpl; intros.
+    constructor.
+    pose proof (IHl _ (refl_equal _) search_term update_term).
+    unfold CountingListAsBag_bdelete in *; simpl in *.
+    destruct (MatchAgainstMany search_term a);
+      destruct (CountingListPartition l (MatchAgainstMany search_term));
+      destruct (List.partition (MatchAgainstMany search_term) l); simpl in *; auto.
+    rewrite Permutation_app_comm; simpl.
+    apply Permutation_cons_app; rewrite Permutation_app_comm; auto.
+  Qed.
 
-    binsert_enumerate := CountingList_BagInsertEnumerate;
-    benumerate_empty  := CountingList_BagEnumerateEmpty;
-    bfind_star        := CountingList_BagFindStar;
-    bfind_correct     := CountingList_BagFindCorrect;
-    bcount_correct    := CountingList_BagCountCorrect;
-    bdelete_correct     := CountingList_BagDeleteCorrect;
-    bupdate_correct     := CountingList_BagUpdateCorrect
-  |}.
+  Instance CountingListAsBag
+  : Bag (CountingList) TItem (list (TItem -> bool)) (TItem -> TItem) :=
+    {|
+      bempty := CountingList_empty;
+      bstar  := nil;
+      bid    := id;
+
+      benumerate := ccontents;
+      bfind      := CountingListAsBag_bfind;
+      binsert    := CountingListAsBag_binsert;
+      bcount     := CountingListAsBag_bcount;
+      bdelete    := CountingListAsBag_bdelete;
+      bupdate    := CountingListAsBag_bupdate;
+
+      binsert_enumerate := CountingList_BagInsertEnumerate;
+      benumerate_empty  := CountingList_BagEnumerateEmpty;
+      bfind_star        := CountingList_BagFindStar;
+      bfind_correct     := CountingList_BagFindCorrect;
+      bcount_correct    := CountingList_BagCountCorrect;
+      bdelete_correct     := CountingList_BagDeleteCorrect;
+      bupdate_correct     := CountingList_BagUpdateCorrect
+    |}.
+
+End CountingListBags.
