src/QueryStructure/Refinements/Bags/ListBags.v
@@ -3,143 +3,129 @@ Unset Implicit Arguments.
 
 Open Scope list.
 
-Definition ListAsBag_bfind 
-           {TItem TSearchTerm: Type}
-           (matcher: TSearchTerm -> TItem -> bool) 
-           (container: list TItem) (search_term: TSearchTerm) :=
-  List.filter (matcher search_term) container.
+Section ListBags.
 
-Definition ListAsBag_binsert 
-           {TItem: Type}
-           (container: list TItem) 
-           (item: TItem) :=
-  cons item container.
+  Context {TItem : Type}
+          {TSearchTerm : Type}
+          {TUpdateTerm : Type}
+          (star: TSearchTerm)
+          (bid : TUpdateTerm)
+          (bfind_matcher: TSearchTerm -> TItem -> bool)
+          (bupdate_transform : TUpdateTerm -> TItem -> TItem)
+          (find_star: forall (i: TItem), bfind_matcher star i = true).
 
-Definition ListAsBag_bcount
-           {TItem TSearchTerm: Type}
-           (matcher: TSearchTerm -> TItem -> bool) 
-           (container: list TItem) (search_term: TSearchTerm) :=
-  List.fold_left (fun acc x => acc + if (matcher search_term x) then 1 else 0) container 0.
+  Definition ListAsBag_bfind
+             (container: list TItem)
+             (search_term: TSearchTerm) :=
+    List.filter (bfind_matcher search_term) container.
 
-Definition ListAsBag_bdelete
-           {TItem TSearchTerm: Type}
-           (bfind_matcher : TSearchTerm -> TItem -> bool)
-           (container : list TItem)
-           (search_term : TSearchTerm) :=
-  snd (List.partition (bfind_matcher search_term) container).
+  Definition ListAsBag_binsert
+             (container: list TItem)
+             (item: TItem) :=
+    cons item container.
 
-Definition ListAsBag_bupdate
-           {TItem TSearchTerm: Type}
-           (bfind_matcher : TSearchTerm -> TItem -> bool)
-           (container : list TItem)
-           (search_term : TSearchTerm) 
-           (f_update : TItem -> TItem) :=
-  (snd (List.partition (bfind_matcher search_term) container))
-       ++ List.map f_update (fst (List.partition (bfind_matcher search_term)
-                                                 container)).
+  Definition ListAsBag_bcount
+             (container: list TItem)
+             (search_term: TSearchTerm) :=
+    List.fold_left (fun acc x => acc + if (bfind_matcher search_term x) then 1 else 0) container 0.
 
-Lemma List_BagInsertEnumerate :
-  forall {TItem: Type},
-  BagInsertEnumerate id (ListAsBag_binsert (TItem := TItem)).
-Proof.
-  firstorder.
-Qed.
+  Definition ListAsBag_bdelete
+             (container : list TItem)
+             (search_term : TSearchTerm) :=
+    List.partition (bfind_matcher search_term) container.
 
-Lemma List_BagEnumerateEmpty :
-  forall {TItem: Type},
+  Definition ListAsBag_bupdate
+             (container   : list TItem)
+             (search_term : TSearchTerm)
+             (update_term : TUpdateTerm) :=
+    (snd (List.partition (bfind_matcher search_term) container))
+      ++ List.map (bupdate_transform update_term)
+      (fst (List.partition (bfind_matcher search_term)
+                           container)).
+
+  Lemma List_BagInsertEnumerate :
+    BagInsertEnumerate id ListAsBag_binsert.
+  Proof.
+    firstorder.
+  Qed.
+
+  Lemma List_BagEnumerateEmpty :
     BagEnumerateEmpty id (@nil TItem).
-Proof.
-  firstorder.
-Qed.
-  
-Lemma List_BagFindStar :
-  forall {TItem TSearchTerm: Type}
-         (star: TSearchTerm)
-         (matcher: TSearchTerm -> TItem -> bool)
-         (find_star: forall (i: TItem), matcher star i = true),
-  BagFindStar (ListAsBag_bfind matcher) id star.
-Proof.
-  intros;
-  induction container; simpl; 
-  [ | rewrite find_star, IHcontainer]; trivial.
-Qed.
+  Proof.
+    firstorder.
+  Qed.
 
-Lemma List_BagFindCorrect :
-  forall {TItem TSearchTerm: Type}
-         (matcher: TSearchTerm -> TItem -> bool),
-         BagFindCorrect (ListAsBag_bfind matcher) matcher id.
-Proof.
-  firstorder.
-Qed.
+  Lemma List_BagFindStar :
+    BagFindStar ListAsBag_bfind id star.
+  Proof.
+    intros;
+    induction container; simpl;
+    [ | rewrite find_star, IHcontainer]; trivial.
+  Qed.
 
-Require Import Omega.
-Lemma List_BagCountCorrect_aux :
-  forall {TItem TSearchTerm: Type}
-         (matcher: TSearchTerm -> TItem -> bool),
-  forall (container: list TItem) (search_term: TSearchTerm) default,
-    length (List.filter (matcher search_term) container) + default =
-    List.fold_left
-      (fun (acc : nat) (x : TItem) =>
-         acc + (if matcher search_term x then 1 else 0)) 
-      container default.
-Proof.
-  induction container; intros.
+  Lemma List_BagFindCorrect :
+    BagFindCorrect ListAsBag_bfind bfind_matcher id.
+  Proof.
+    firstorder.
+  Qed.
 
-  + trivial.
-  + simpl; destruct (matcher search_term a);
-    simpl; rewrite <- IHcontainer; omega. 
-Qed.
+  Require Import Omega.
+  Lemma List_BagCountCorrect_aux :
+    forall (container: list TItem) (search_term: TSearchTerm) default,
+      length (List.filter (bfind_matcher search_term) container) + default =
+      List.fold_left
+        (fun (acc : nat) (x : TItem) =>
+           acc + (if bfind_matcher search_term x then 1 else 0))
+        container default.
+  Proof.
+    induction container; intros.
 
-Lemma List_BagCountCorrect :
-  forall {TItem TSearchTerm: Type}
-         (matcher: TSearchTerm -> TItem -> bool),
-         BagCountCorrect (ListAsBag_bcount matcher) (ListAsBag_bfind matcher).
-Proof.
-  unfold BagCountCorrect, ListAsBag_bcount, ListAsBag_bfind; intros;
-  pose proof (List_BagCountCorrect_aux matcher container search_term 0) as temp;
-  rewrite plus_0_r in temp; simpl in temp; exact temp.
-Qed.
+    + trivial.
+    + simpl; destruct (bfind_matcher search_term a);
+      simpl; rewrite <- IHcontainer; omega.
+  Qed.
 
-Lemma List_BagDeleteCorrect :
-  forall {TItem TSearchTerm: Type}
-         (matcher: TSearchTerm -> TItem -> bool),
-    BagDeleteCorrect (ListAsBag_bfind matcher) matcher id
-                     (ListAsBag_bdelete matcher).
-Proof.
-  firstorder.
-Qed.
+  Lemma List_BagCountCorrect :
+    BagCountCorrect ListAsBag_bcount ListAsBag_bfind.
+  Proof.
+    unfold BagCountCorrect, ListAsBag_bcount, ListAsBag_bfind; intros;
+    pose proof (List_BagCountCorrect_aux container search_term 0) as temp;
+    rewrite plus_0_r in temp; simpl in temp; exact temp.
+  Qed.
 
-Lemma List_BagUpdateCorrect :
-  forall {TItem TSearchTerm: Type}
-         (matcher: TSearchTerm -> TItem -> bool),
-    BagUpdateCorrect (ListAsBag_bfind matcher) matcher id
-   (ListAsBag_bupdate matcher).
-Proof.
-  firstorder.
-Qed.
+  Lemma List_BagDeleteCorrect :
+    BagDeleteCorrect ListAsBag_bfind bfind_matcher id ListAsBag_bdelete.
+  Proof.
+    firstorder.
+  Qed.
 
-Instance ListAsBag
-         {TItem TSearchTerm: Type}
-         (star: TSearchTerm)
-         (matcher: TSearchTerm -> TItem -> bool)
-         (find_star: forall (i: TItem), matcher star i = true)
-: Bag (list TItem) TItem TSearchTerm :=
-  {| 
-    bempty := nil;
-    bstar  := star;
-    
-    benumerate := id;
-    bfind      := ListAsBag_bfind matcher;
-    binsert    := ListAsBag_binsert;
-    bcount     := ListAsBag_bcount matcher;
-    bdelete    := ListAsBag_bdelete matcher;
-    bupdate    := ListAsBag_bupdate matcher;
+  Lemma List_BagUpdateCorrect :
+    BagUpdateCorrect ListAsBag_bfind bfind_matcher id bupdate_transform ListAsBag_bupdate.
+  Proof.
+    firstorder.
+  Qed.
 
-    binsert_enumerate := List_BagInsertEnumerate;
-    benumerate_empty  := List_BagEnumerateEmpty;
-    bfind_star        := List_BagFindStar star matcher find_star;
-    bfind_correct     := List_BagFindCorrect matcher;
-    bcount_correct    := List_BagCountCorrect matcher;
-    bdelete_correct   := List_BagDeleteCorrect matcher;
-    bupdate_correct   := List_BagUpdateCorrect matcher
-  |}.
+  Global Instance ListAsBag
+  : Bag (list TItem) TItem TSearchTerm TUpdateTerm :=
+    {|
+      bempty := nil;
+      bid    := bid;
+      bstar  := star;
+
+      benumerate := id;
+      bfind      := ListAsBag_bfind;
+      binsert    := ListAsBag_binsert;
+      bcount     := ListAsBag_bcount;
+      bdelete    := ListAsBag_bdelete;
+      bupdate    := ListAsBag_bupdate;
+
+      binsert_enumerate := List_BagInsertEnumerate;
+      benumerate_empty  := List_BagEnumerateEmpty;
+      bfind_star        := List_BagFindStar;
+      bfind_correct     := List_BagFindCorrect;
+      bcount_correct    := List_BagCountCorrect;
+      bdelete_correct   := List_BagDeleteCorrect;
+      bupdate_correct   := List_BagUpdateCorrect
+    |}.
+
+End ListBags.
